ulib/tactics_ml/FStar_Tactics_Builtins.ml
@@ -181,6 +181,7 @@ let check_subtyping         = from_tac_3 B.refl_check_subtyping
 let check_equiv             = from_tac_3 B.refl_check_equiv
 let tc_term                 = from_tac_2 B.refl_tc_term
 let universe_of             = from_tac_2 B.refl_universe_of
+let check_prop_validity     = from_tac_2 B.refl_check_prop_validity
 
 (* The handlers need to "embed" their argument. *)
 let catch   (t: unit -> 'a __tac): ((exn, 'a) either) __tac = from_tac_1 TM.catch   (to_tac_0 (t ()))
