src/tactics/FStar.Tactics.Basic.fsti
@@ -118,8 +118,9 @@ val term_eq_old            : term -> term -> tac bool
 val with_compat_pre_core   : Z.t -> tac 'a -> tac 'a
 
 (*****)
-val refl_check_subtyping : env -> typ -> typ -> tac (option unit)
-val refl_check_equiv     : env -> typ -> typ -> tac (option unit)
-val refl_tc_term         : env -> term -> tac (option typ)
-val refl_universe_of     : env -> term -> tac (option universe)
+val refl_check_subtyping     : env -> typ -> typ -> tac (option unit)
+val refl_check_equiv         : env -> typ -> typ -> tac (option unit)
+val refl_tc_term             : env -> term -> tac (option typ)
+val refl_universe_of         : env -> term -> tac (option universe)
+val refl_check_prop_validity : env -> term -> tac (option unit)
 
